all but univ elim

MCA.v
@@ -44,64 +44,201 @@ subs (var (FS x)) c := var x;
 subs (cst c') c := cst c';
 subs (eapp e e') c := eapp (subs e c) (subs e' c).
 
-(*Fixpoint fin n : Type :=
-  match n with 0 => False | S n => option (fin n) end.
-
-Inductive exp {M : Monad} {mas : MAS M} : nat -> Type :=
-| var n : fin n -> exp n
-| cst {n} : code -> exp n
-| eapp n : exp n -> exp n -> exp n.
-
-Equations subs {M : Monad} {mas : MAS M} n (e : exp (S n)) (c : code) : exp n :=
-subs (var None) c := cst c;
-subs (var (Some x)) c := var x;
-subs (cst c') c := cst c';
-subs (eapp e e') c := eapp (subs e c) (subs e' c).*)
-
 Equations eval {M : Monad} {mas : MAS M} (e : exp 0) : M code :=
 eval (cst c) := ret c;
 eval (eapp e e') := bind (eval e) (fun cf => bind (eval e') (fun ca => mapp cf ca)).
 
-Class MCA (M : Monad) :=
+Class MCA (M : Monad) (mas : MAS M) :=
 {
-  mca_mas : MAS M;
   lam n : exp (S n) -> code;
 
   lam_S n (e : exp (S (S n))) c : mapp (lam e) c = ret (lam (subs e c));
   lam_O (e : exp 1) c : mapp (lam e) c = eval (subs e c);
 }.
 
+Arguments lam {_ _ _} _ _.
 
 
-(* PCAs *)
 
-Definition subsingleton A :=
-  { P : A -> Prop | forall x y, P x -> P y -> x = y }.
+(* Evidenced Frames *)
 
-Lemma subsingleton_eq A (P Q : subsingleton A) :
-  (forall x, proj1_sig P x <-> proj1_sig Q x) -> P = Q.
+Class EF : Type :=
+{
+  prop : Type;
+  evid : Type;
+  erel : prop -> evid -> prop -> Prop;
+
+  top : prop;
+  conj : prop -> prop -> prop;
+  uimp : prop -> (prop -> Prop) -> prop;
+
+  eid : evid;
+  eseq : evid -> evid -> evid;
+  etop : evid;
+  epair : evid -> evid -> evid;
+  efst : evid;
+  esnd : evid;
+  elam : evid -> evid;
+  erho : evid -> evid;
+
+  ef_refl phi : erel phi eid phi;
+  ef_trans phi1 phi2 phi3 e e' : erel phi1 e phi2 -> erel phi2 e' phi3 -> erel phi1 (eseq e e') phi3;
+  ef_top phi : erel phi etop top;
+  ef_pair phi psi psi' e e' : erel phi e psi -> erel phi e' psi' -> erel phi (epair e e') (conj psi psi');
+  ef_fst phi psi : erel (conj phi psi) efst phi;
+  ef_snd phi psi : erel (conj phi psi) esnd psi;
+  ef_curry phi phi' P e : (forall psi, P psi -> erel (conj phi phi') e psi) -> erel phi (elam e) (uimp phi' P);
+  ef_uncurry phi phi' P e psi : erel phi (elam e) (uimp phi' P) -> P psi -> erel (conj phi phi') (erho e) psi;
+}.
+
+
+
+(* M-Modalities *)
+
+Class MMod (M : Monad) (mas : MAS M) (mca : MCA mas) : Type :=
+{
+  Omega : Type;
+  hrel : Omega -> Omega -> Prop;
+  htop : Omega;
+  hmeet : Omega -> Omega -> Omega;
+  himp : Omega -> Omega -> Omega;
+  hinf : (Omega -> Prop) -> Omega;
+
+  after A : M A -> (A -> Omega) -> Omega;
+
+  ax_refl x : hrel x x;
+  ax_trans x y z : hrel x y -> hrel y z -> hrel x z;
+  ax_top x : hrel x htop;
+  ax_meet1 x y : hrel (hmeet x y) x;
+  ax_meet2 x y : hrel (hmeet x y) y;
+  ax_meet x y z : hrel z x -> hrel z y -> hrel z (hmeet x y);
+  ax_imp x y z : hrel (hmeet x y) z <-> hrel x (himp y z);
+  ax_inf P x : (forall y, P y -> hrel x y) <-> hrel x (hinf P);
+
+  ax_ret A x (phi : A -> Omega) : hrel (phi x) (after (ret x) phi);
+  ax_bind A B (f : A -> M B) phi m : hrel (after m (fun x => after (f x) phi)) (after (bind m f) phi);
+  ax_mono_ext A (phi psi : A -> Omega) m : (forall c, hrel (phi c) (psi c)) -> hrel (after m phi) (after m psi);
+  ax_mono_meet A (phi : A -> Omega) m x : hrel (hmeet x (after m phi)) (after m (fun a => hmeet x (phi a)));
+}.
+
+Add Parametric Relation M (mas : MAS M) (mca : MCA mas) (mod : MMod mca) :
+  Omega hrel
+  reflexivity proved by ax_refl
+  transitivity proved by ax_trans
+  as hrel_instance.
+
+Notation "x <= y" := (hrel x y).
+
+Definition ihinf M (mas : MAS M) (mca : MCA mas) (mod : MMod mca) :
+  forall I, (I -> Omega) -> Omega :=  
+  fun I F => hinf (fun o => exists i, o = F i).
+
+Definition ax_refl' M (mas : MAS M) (mca : MCA mas) (mod : MMod mca) x x' :
+  x = x' -> x <= x'.
 Proof.
-Admitted.
+  intros <-. apply ax_refl.
+Qed.
 
-Definition partiality_monad : Monad.
+Definition ax_meet_comm M (mas : MAS M) (mca : MCA mas) (mod : MMod mca) x y :
+  hmeet x y <= hmeet y x.
 Proof.
-  unshelve eapply (Build_Monad (M := subsingleton)).
-  - intros A x. exists (eq x). intros y y' ->. tauto.
-  - intros A B [P HP] F. exists (fun b => exists a, P a /\ proj1_sig (F a) b).
-    intros x y [a [H1 H2]] [a' [H3 H4]]. apply (HP a a') in H1 as <-; trivial.
-    destruct (F a) as [Q HQ]. cbn in *. now apply HQ.
-  - intros A [P HP]. cbn. apply subsingleton_eq. cbn.
-    intros x. split; eauto. intros [y [H ->]]. assumption.
-  - intros A B f x. apply subsingleton_eq. cbn.
-    intros y. split; eauto. intros [z [-> H]]. assumption.
-  - intros A B C f g [P HP]. apply subsingleton_eq. cbn.
-    intros c. split.
-    + intros (b & (a & H1 & H2) & H3). exists a. split; trivial.
-      destruct (f a) as [Q HQ]. cbn in *. now exists b.
-    + intros (a & H1 & H2). destruct (f a) as [Q HQ] eqn: He. cbn in H2.
-      destruct H2 as (b & H3 & H4). exists b. split; trivial.
-      exists a. rewrite He. cbn. split; trivial.
-Defined.
+  apply ax_meet. apply ax_meet2. apply ax_meet1.
+Qed.
 
 
 
+(* Induced EF *)
+
+Notation "$0" :=
+  (var F1).
+
+Notation "$1" :=
+  (var (FS F1)).
+
+Notation "$2" :=
+  (var (FS (FS F1))).
+
+Notation p1 :=
+  (lam 1 $0).
+
+Notation p2 :=
+  (lam 1 $1).
+
+Theorem MCA_EF M (mas : MAS M) (mca : MCA mas) (mod : MMod mca) : EF.
+Proof.
+  unshelve econstructor.
+  - exact (code -> Omega).
+  - exact code.
+  - exact (fun P e P' => forall c, P c <= after (mapp e c) P').
+  - exact (fun _ => htop).
+  - intros P P' e. exact (hmeet (after (mapp e p1) P) (after (mapp e p2) P')).
+  - intros P P' e. apply hinf. intros o.
+    exact (exists c phi, P' phi /\ o = himp (P c) (after (mapp e c) phi)).
+  - exact (lam 0 $0).
+  - intros f g. exact (lam 0 (eapp (cst g) (eapp (cst f) $0))).
+  - exact (lam 0 $0).
+  - intros e e'. exact (lam 1 (eapp (eapp $1 (eapp (cst e) $0)) (eapp (cst e') $0))).
+  - exact (lam 0 (eapp $0 (cst p1))).
+  - exact (lam 0 (eapp $0 (cst p2))).
+  - intros e. exact (lam 1 (eapp (cst e) (eapp (eapp (cst (lam 2 (eapp (eapp $2 $0) $1))) $0) $1))).
+  - intros e. exact (lam 0 (eapp (eapp (cst e) (eapp $0 (cst p1))) (eapp $0 (cst p2)))).
+  - cbn. intros phi c. rewrite lam_O. autorewrite with subs eval. apply ax_ret.
+  - cbn. intros phi1 phi2 phi3 e e' H1 H2 c.
+    rewrite !lam_O. autorewrite with subs eval.
+    rewrite !lunit. rewrite <- ax_bind, H1.
+    apply ax_mono_ext. apply H2.
+  - cbn. intros phi c. rewrite lam_O.
+    autorewrite with subs eval.
+    rewrite <- ax_ret; eauto. apply ax_top.
+  - cbn. intros phi psi psi' e e' H1 H2 c.
+    assert (HC : phi c <= after (mapp e c) (fun c1 => after (mapp e' c) (fun c2 => hmeet (psi c1) (psi' c2)))).
+    { rewrite <- ax_mono_ext. rewrite <- ax_mono_meet.
+      apply ax_meet. apply H2. apply H1. intros m. cbn.
+      rewrite ax_meet_comm. apply ax_mono_meet. }
+    assert (HC1 : phi c <= after (mapp e c) (fun c1 => after (mapp e' c) (fun c2 => psi c1))).
+    { rewrite HC. apply ax_mono_ext. intros m. apply ax_mono_ext. intros m'. apply ax_meet1. }
+    assert (HC2 : phi c <= after (mapp e c) (fun c1 => after (mapp e' c) (fun c2 => psi' c2))).
+    { rewrite HC. apply ax_mono_ext. intros m. apply ax_mono_ext. intros m'. apply ax_meet2. }
+    rewrite !lam_S. autorewrite with subs eval. rewrite <- ax_ret.
+    rewrite !lam_O. autorewrite with subs eval.
+    rewrite !lunit, !assoc. apply ax_meet.
+    + rewrite <- ax_bind. rewrite HC1. apply ax_mono_ext.
+      intros x. rewrite !lam_S. autorewrite with subs eval. rewrite lunit.
+      rewrite <- ax_bind. apply ax_mono_ext. intros m.
+      rewrite lam_O. autorewrite with subs eval. apply ax_ret.
+    + rewrite <- ax_bind. rewrite HC2. apply ax_mono_ext.
+      intros x. rewrite !lam_S. autorewrite with subs eval. rewrite lunit.
+      rewrite <- ax_bind. apply ax_mono_ext. intros m.
+      rewrite lam_O. autorewrite with subs eval. apply ax_ret.
+  - cbn. intros phi psi c.
+    rewrite lam_O. autorewrite with subs eval.
+    rewrite <- ax_bind, <- ax_ret, <- ax_bind, <- ax_ret.
+    apply ax_meet1.
+  - cbn. intros phi psi c.
+    rewrite lam_O. autorewrite with subs eval.
+    rewrite <- ax_bind, <- ax_ret, <- ax_bind, <- ax_ret.
+    apply ax_meet2.
+  - cbn. intros phi psi P c H c'.
+    rewrite lam_S. autorewrite with subs eval.
+    rewrite <- ax_ret. apply ax_inf.
+    intros x (m & phi' & HP & ->).
+    rewrite lam_O. autorewrite with subs eval.
+    rewrite lunit. apply ax_imp. rewrite <- !ax_bind, <- ax_ret, <- ax_bind, <- ax_ret.
+    rewrite lam_S. autorewrite with subs eval.
+    rewrite <- ax_ret. rewrite lunit.
+    rewrite lam_S. autorewrite with subs eval.
+    rewrite <- ax_ret.
+    rewrite <- H; trivial.
+    rewrite !lam_O. autorewrite with subs eval. apply ax_meet.
+    + rewrite <- !ax_bind, <- ax_ret, lunit.
+      rewrite lam_S. autorewrite with subs eval.
+      rewrite <- ax_ret, lunit.
+      rewrite lam_O. autorewrite with subs eval.
+      rewrite <- ax_ret. apply ax_meet1.
+    + rewrite <- !ax_bind, <- ax_ret, lunit.
+      rewrite lam_S. autorewrite with subs eval.
+      rewrite <- ax_ret, lunit.
+      rewrite lam_O. autorewrite with subs eval.
+      rewrite <- ax_ret. apply ax_meet2.
+  - cbn.
+Qed.
